src/protocol/DNS.Protocol.Parser.EverParseAdapter.fst
@@ -26,6 +26,8 @@ let generated_dns_uncompressed_question_aaaa_answer_packet_validator_linked : bo
 
 let generated_dns_uncompressed_question_name_rdata_answer_packet_validator_linked : bool = true
 
+let generated_dns_uncompressed_question_mx_answer_packet_validator_linked : bool = true
+
 let generated_dns_header_validator = DNSProtocol.validate__dns_header
 
 let generated_dns_root_question_validator =
@@ -56,3 +58,10 @@ let generated_dns_uncompressed_question_name_rdata_answer_packet_validator
     rr_name_length
     rdata_name_length
     expected_rtype
+
+let generated_dns_uncompressed_question_mx_answer_packet_validator
+    qname_length rr_name_length exchange_name_length =
+  DNSProtocol.validate__dns_uncompressed_question_mx_answer_packet
+    qname_length
+    rr_name_length
+    exchange_name_length
